L20 interpreter is now split the same way as L10

L20/Interpret.v
@@ -1,6 +1,8 @@
 From Coq Require Import String Arith NArith ZArith.
-From Vyper Require Import Config L20.AST L20.Callset.
-From Vyper Require FSet Map L10.AST L10.UInt256.
+From Vyper Require Import Config Calldag.
+From Vyper.L10 Require Import Base.
+From Vyper.L20 Require Import AST Callset Descend Expr Stmt.
+From Vyper Require FSet Map L10.UInt256 L10.Interpret.
 
 Local Open Scope list_scope.
 Local Open Scope string_scope.
@@ -8,40 +10,6 @@ Local Open Scope string_scope.
 Section Interpret.
 
 Context {C: VyperConfig}.
-
-Definition abort := L10.Interpret.abort.
-Definition expr_result := L10.Interpret.expr_result.
-Definition stmt_result := L10.Interpret.stmt_result.
-Definition expr_error {type: Type} := @L10.Interpret.expr_error C type.
-
-Definition calldag := L10.Interpret.generic_calldag decl decl_callset.
-Definition cd_declmap {C decl_type callset} := @L10.Interpret.cd_declmap C decl_type callset.
-Definition cd_depthmap {C decl_type callset} := @L10.Interpret.cd_depthmap C decl_type callset.
-Definition cd_depthmap_ok {C decl_type callset} := @L10.Interpret.cd_depthmap_ok C decl_type callset.
-
-
-(** Initialize a map of local variables with argument names and argument values. *)
-Fixpoint bind_args (names: list string) (values: list uint256)
-: string + string_map uint256
-:= let _ := string_map_impl in
-   match names with
-   | nil => match values with
-            | nil => inr Map.empty
-            | _ => inl "function called with too many arguments"
-            end
-   | hn :: tn => match values with
-                 | nil => inl "function called with too few arguments"
-                 | hv :: tv =>
-                     match bind_args tn tv with
-                     | inl err => inl err
-                     | inr bindings =>
-                        match Map.lookup bindings hn with
-                        | Some _ => inl "error: duplicate variable name"
-                        | None => inr (Map.insert bindings hn hv)
-                        end
-                     end
-                 end
-   end.
 
 Local Lemma interpret_call_helper {this_decl: decl}
                                   {fun_name: string}
@@ -53,467 +21,15 @@ Proof.
 subst this_decl. unfold decl_callset. apply FSet.is_subset_refl.
 Qed.
 
-(* XXX dup from L10 except PrivateOrBuiltinCall becomes PrivateCall *)
-Lemma call_descend {call_depth_bound new_call_depth_bound current_fun_depth: nat}
-                   (DepthOk : current_fun_depth < call_depth_bound)
-                   (cd : calldag)
-                   (this_fun_name: string)
-                   (this_decl: decl)
-                   (this_decl_ok: cd_declmap cd this_fun_name = Some this_decl)
-                   (current_fun_depth_ok:
-                     cd_depthmap cd this_fun_name = Some current_fun_depth)
-                   (e: expr)
-                   (CallOk : let _ := string_set_impl in
-                             FSet.is_subset (expr_callset e) (decl_callset this_decl) = true)
-                   (Ebound : call_depth_bound = S new_call_depth_bound)
-                   (name : string)
-                   (args : list expr)
-                   (E : e = PrivateCall name args)
-                   {depth: nat}
-                   (Edepth: cd_depthmap cd name = Some depth):
-  depth < new_call_depth_bound.
-Proof.
-subst e. cbn in CallOk.
-assert(HasName: let _ := string_set_impl in FSet.has (decl_callset this_decl) name = true).
-{
-  cbn.
-  apply (FSet.is_subset_if CallOk name).
-  apply FSet.add_has.
-}
-clear CallOk. cbn in HasName.
-assert (K := cd_depthmap_ok cd this_fun_name).
-unfold cd_declmap in this_decl_ok. rewrite this_decl_ok in K.
-unfold cd_depthmap in current_fun_depth_ok. rewrite current_fun_depth_ok in K.
-cbn in K.
-rewrite FSet.for_all_ok in K.
-assert (L := K name HasName). clear K.
-subst call_depth_bound.
-apply lt_n_Sm_le in DepthOk.
-unfold cd_depthmap in Edepth.
-rewrite Edepth in L.
-destruct current_fun_depth. { discriminate. }
-rewrite Nat.leb_le in L.
-rewrite Nat.le_succ_l in DepthOk.
-apply (Nat.le_lt_trans _ _ _ L DepthOk).
-Qed.
-
-Record fun_ctx (cd: calldag) (bound: nat) := {
-  fun_name: string;
-  fun_depth: nat;
-  fun_depth_ok: cd_depthmap cd fun_name = Some fun_depth;
-  fun_decl: decl;
-  fun_decl_ok: cd_declmap cd fun_name = Some fun_decl;
-  fun_bound_ok: fun_depth < bound;
-}.
-Arguments fun_name     {_ _}.
-Arguments fun_depth    {_ _}.
-Arguments fun_depth_ok {_ _}.
-Arguments fun_decl     {_ _}.
-Arguments fun_decl_ok  {_ _}.
-Arguments fun_bound_ok {_ _}.
-
-Local Lemma fun_ctx_descend_helper {cd: calldag}
-                                   {name: string}
-                                   {d: decl}
-                                   (Edecl : cd_declmap cd name = Some d):
-  cd_depthmap cd name <> None.
-Proof.
-assert (D := cd_depthmap_ok cd name).
-unfold cd_declmap in Edecl.
-rewrite Edecl in D.
-intro H.
-unfold cd_depthmap in H.
-rewrite H in D.
-exact D.
-Qed.
-
-(** Make a callee context from a caller context and a call expression, 
-  The None result means that no declaration with the given name is found.
-  No check is made that the callee context is indeed a function.
-  The max stack depth bound is reduced by 1.
- *)
-Definition fun_ctx_descend {call_depth_bound new_call_depth_bound}
-                           {cd: calldag}
-                           {e: expr}
-                           {name: string}
-                           {args: list expr}
-
-                           (fc: fun_ctx cd call_depth_bound)
-                           (CallOk: let _ := string_set_impl in
-                                       FSet.is_subset (expr_callset e)
-                                                      (decl_callset (fun_decl fc))
-                                        = true)
-                           (Ebound: call_depth_bound = S new_call_depth_bound)
-                           (E: e = PrivateCall name args)
-: option (fun_ctx cd new_call_depth_bound)
-:= match cd_declmap cd name as maybe_decl return _ = maybe_decl -> _ with
-   | None => fun _ =>
-       (* no declaration found - could be a builtin *)
-       None
-   | Some d => fun Edecl =>
-       match cd_depthmap cd name as maybe_depth return _ = maybe_depth -> _ with
-       | None => fun Edepth => False_rect _ (fun_ctx_descend_helper Edecl Edepth)
-       | Some depth => fun Edepth =>
-           Some {| fun_name := name
-                 ; fun_depth := depth
-                 ; fun_depth_ok := Edepth
-                 ; fun_decl := d
-                 ; fun_decl_ok := Edecl
-                 ; fun_bound_ok := call_descend (fun_bound_ok fc) cd (fun_name fc)
-                                                (fun_decl fc) (fun_decl_ok fc)
-                                                (fun_depth_ok fc) e CallOk Ebound 
-                                                name args E Edepth
-                |}
-       end eq_refl
-   end eq_refl.
-
 (*************************************************************************************************)
 
 Definition map_lookup {Value} (m: string_map Value) := let _ := string_map_impl in Map.lookup m.
 Definition map_insert {Value} (m: string_map Value) := let _ := string_map_impl in Map.insert m.
 Definition map_remove {Value} (m: string_map Value) := let _ := string_map_impl in Map.remove m.
 
-Fixpoint interpret_expr {bigger_call_depth_bound smaller_call_depth_bound: nat}
-                        (Ebound: bigger_call_depth_bound = S smaller_call_depth_bound)
-                        {cd: calldag}
-                        (fc: fun_ctx cd bigger_call_depth_bound)
-                        (do_call: forall
-                                      (fc': fun_ctx cd smaller_call_depth_bound)
-                                      (world: world_state)
-                                      (arg_values: list uint256),
-                                    world_state * expr_result uint256)
-                        (builtins: string -> option L10.Interpret.builtin)
-                        (world: world_state)
-                        (loc: string_map uint256)
-                        (e: expr)
-                        (CallOk: let _ := string_set_impl in 
-                                   FSet.is_subset (expr_callset e)
-                                                  (decl_callset (fun_decl fc))
-                                   = true)
-{struct e}
-: world_state * expr_result uint256
-:= let fix interpret_expr_list (world: world_state)
-                               (loc: string_map uint256)
-                               (e: list expr)
-                               (CallOk: let _ := string_set_impl in 
-                                        FSet.is_subset (expr_list_callset e)
-                                                       (decl_callset (fun_decl fc))
-                                        = true)
-      {struct e}
-      : world_state * expr_result (list uint256)
-      := match e as e' return e = e' -> _ with
-         | nil => fun _ => (world, L10.Interpret.ExprSuccess _ nil)
-         | (h :: t)%list => fun E =>
-             let (world', result_h) := interpret_expr Ebound fc do_call builtins
-                                                      world loc h
-                                                      (callset_descend_head E CallOk)
-             in match result_h with
-                | L10.Interpret.ExprAbort _ ab => (world', L10.Interpret.ExprAbort _ ab)
-                | L10.Interpret.ExprSuccess _ x =>
-                   let (world'', result_t) := interpret_expr_list world' loc t
-                                                                  (callset_descend_tail E CallOk)
-                   in (world'', match result_t with
-                                | L10.Interpret.ExprAbort _ _ => result_t
-                                | L10.Interpret.ExprSuccess _ y => 
-                                    L10.Interpret.ExprSuccess _ (x :: y)%list
-                                end)
-                 end
-         end eq_refl
-    in match e as e' return e = e' -> _ with
-       | Const val => fun _ => (world, L10.Interpret.ExprSuccess _ val)
-       | LocalVar name => fun _ =>
-           (world, match map_lookup loc name with
-                   | Some val => L10.Interpret.ExprSuccess _ val
-                   | None => expr_error "Local variable not found"
-                   end)
-       | StorageVar name => fun _ => 
-           (world, match storage_lookup world name with
-                   | Some val => L10.Interpret.ExprSuccess _ val
-                   | None => expr_error "Storage variable not found"
-                   end)
-       | UnOp op a => fun E =>
-           let (world', result) := interpret_expr Ebound fc do_call builtins
-                                                  world loc a
-                                                  (callset_descend_unop E CallOk)
-           in (world', match result with
-                       | L10.Interpret.ExprSuccess _ val => L10.Interpret.interpret_unop op val
-                       | L10.Interpret.ExprAbort _ _ => result
-                       end)
-       | BinOp op a b => fun E =>
-           let (world', result_a) := interpret_expr Ebound fc do_call builtins
-                                                    world loc a
-                                                    (callset_descend_binop_left E CallOk)
-           in match result_a with
-           | L10.Interpret.ExprAbort _ _ => (world', result_a)
-           | L10.Interpret.ExprSuccess _ x =>
-             let (world'', result_b) := interpret_expr Ebound fc do_call builtins
-                                                       world' loc b
-                                                       (callset_descend_binop_right E CallOk)
-             in (world'', match result_b with
-                          | L10.Interpret.ExprAbort _ _ => result_b
-                          | L10.Interpret.ExprSuccess _ y => L10.Interpret.interpret_binop op x y
-                          end)
-           end
-       | IfThenElse cond yes no => fun E =>
-           let (world', result_cond) := interpret_expr Ebound fc do_call builtins
-                                                       world loc cond
-                                                       (callset_descend_if_cond E CallOk)
-           in match result_cond with
-              | L10.Interpret.ExprAbort _ _ => (world', result_cond)
-              | L10.Interpret.ExprSuccess _ cond_value =>
-                  if (Z_of_uint256 cond_value =? 0)%Z
-                    then interpret_expr Ebound fc do_call builtins
-                                        world' loc no
-                                        (callset_descend_if_else E CallOk)
-                    else interpret_expr Ebound fc do_call builtins
-                                        world' loc yes
-                                        (callset_descend_if_then E CallOk)
-              end
-       | LogicalAnd a b => fun E =>
-           let (world', result_a) := interpret_expr Ebound fc do_call builtins
-                                                    world loc a
-                                                    (callset_descend_and_left E CallOk)
-           in match result_a with
-              | L10.Interpret.ExprAbort _ _ => (world', result_a)
-              | L10.Interpret.ExprSuccess _ a_value =>
-                  if (Z_of_uint256 a_value =? 0)%Z
-                    then (world', result_a)
-                    else interpret_expr Ebound fc do_call builtins
-                                        world' loc b
-                                        (callset_descend_and_right E CallOk)
-              end
-       | LogicalOr a b => fun E =>
-           let (world', result_a) := interpret_expr Ebound fc do_call builtins
-                                                    world loc a
-                                                    (callset_descend_or_left E CallOk)
-           in match result_a with
-              | L10.Interpret.ExprAbort _ msg => (world', result_a)
-              | L10.Interpret.ExprSuccess _ a_value =>
-                  if (Z_of_uint256 a_value =? 0)%Z
-                    then interpret_expr Ebound fc do_call builtins
-                                        world' loc b
-                                        (callset_descend_or_right E CallOk)
-                    else (world', result_a)
-              end
-       | PrivateCall name args => fun E =>
-           let (world', result_args) :=
-             interpret_expr_list world loc args
-                                 (callset_descend_args E CallOk)
-           in match result_args with
-              | L10.Interpret.ExprAbort _ ab => (world', L10.Interpret.ExprAbort _ ab)
-              | L10.Interpret.ExprSuccess _ arg_values =>
-                  match fun_ctx_descend fc CallOk Ebound E with
-                  | None => (* can't resolve the function, maybe it's a builtin *)
-                            (world', expr_error "can't resolve function name")
-                  | Some new_fc => do_call new_fc world' arg_values
-                  end
-              end
-       | BuiltinCall name args => fun E =>
-           let (world', result_args) :=
-             interpret_expr_list world loc args
-                                 (callset_descend_builtin_args E CallOk)
-           in match result_args with
-              | L10.Interpret.ExprAbort _ ab => (world', L10.Interpret.ExprAbort _ ab)
-              | L10.Interpret.ExprSuccess _ arg_values =>
-                match builtins name with
-                | Some (existT _ arity b) =>
-                   (if (arity =? List.length arg_values)%nat as arity_ok 
-                    return _ = arity_ok -> _
-                        then fun Earity =>
-                               L10.Interpret.call_builtin arg_values Earity (b world')
-                        else fun _ => (world', expr_error "builtin with wrong arity"))
-                      eq_refl
-                | None => (world', expr_error "can't resolve function name")
-                end
-              end
-       end eq_refl.
-
-Definition interpret_small_stmt {bigger_call_depth_bound smaller_call_depth_bound: nat}
-                                (Ebound: bigger_call_depth_bound = S smaller_call_depth_bound)
-                                {cd: calldag}
-                                (fc: fun_ctx cd bigger_call_depth_bound)
-                                (do_call: forall
-                                              (fc': fun_ctx cd smaller_call_depth_bound)
-                                              (world: world_state)
-                                              (arg_values: list uint256),
-                                            world_state * expr_result uint256)
-                                (builtins: string -> option L10.Interpret.builtin)
-                                (world: world_state)
-                                (loc: string_map uint256)
-                                (s: small_stmt)
-                                (CallOk: let _ := string_set_impl in 
-                                         FSet.is_subset (small_stmt_callset s)
-                                                        (decl_callset (fun_decl fc))
-                                         = true)
-: world_state * string_map uint256 * stmt_result uint256
-:= match s as s' return s = s' -> _ with
-   | Pass     => fun _ => (world, loc, L10.Interpret.StmtSuccess _)
-   | Abort ab => fun _ => (world, loc, L10.Interpret.StmtAbort _ ab)
-   | Return e => fun E =>
-        let (world', result) := interpret_expr Ebound fc do_call builtins
-                                               world loc e
-                                               (callset_descend_return E CallOk)
-        in (world', loc, match result with
-                         | L10.Interpret.ExprSuccess _ value =>
-                              L10.Interpret.StmtReturnFromFunction _ value
-                         | L10.Interpret.ExprAbort _ ab =>
-                              L10.Interpret.StmtAbort _ ab
-                         end)
-   | Raise e => fun E =>
-        let (world', result) := interpret_expr Ebound fc do_call builtins
-                                               world loc e
-                                               (callset_descend_raise E CallOk)
-        in (world', loc, L10.Interpret.StmtAbort _
-                           (match result with
-                            | L10.Interpret.ExprSuccess _ value =>
-                                L10.Interpret.AbortException value
-                            | L10.Interpret.ExprAbort _ ab => ab
-                            end))
-   | Assign lhs rhs => fun E =>
-        let (world', result) := interpret_expr Ebound fc do_call builtins
-                                               world loc rhs
-                                               (callset_descend_assign_rhs E CallOk)
-        in L10.Interpret.do_assign world' loc lhs result
-   | ExprStmt e => fun E =>
-                   let (world', result) := interpret_expr Ebound fc do_call builtins
-                                                          world loc e
-                                                          (callset_descend_expr_stmt E CallOk)
-                   in (world', loc, match result with
-                                    | L10.Interpret.ExprSuccess _ a =>
-                                        L10.Interpret.StmtSuccess _
-                                    | L10.Interpret.ExprAbort _ ab =>
-                                        L10.Interpret.StmtAbort _ ab
-                                    end)
-   end eq_refl.
-
-Fixpoint interpret_stmt {bigger_call_depth_bound smaller_call_depth_bound: nat}
-                        (Ebound: bigger_call_depth_bound = S smaller_call_depth_bound)
-                        {cd: calldag}
-                        (fc: fun_ctx cd bigger_call_depth_bound)
-                        (do_call: forall
-                                      (fc': fun_ctx cd smaller_call_depth_bound)
-                                      (world: world_state)
-                                      (arg_values: list uint256),
-                                    world_state * expr_result uint256)
-                        (builtins: string -> option L10.Interpret.builtin)
-                        (world: world_state)
-                        (loc: string_map uint256)
-                        (s: stmt)
-                        (CallOk: let _ := string_set_impl in 
-                                 FSet.is_subset (stmt_callset s)
-                                                (decl_callset (fun_decl fc)) = true)
- {struct s}
- : world_state * string_map uint256 * stmt_result uint256
- := match s as s' return s = s' -> _ with
-    | Semicolon a b => fun E =>
-         let '(world', loc', result_a) :=
-                interpret_stmt Ebound fc do_call builtins
-                               world loc a
-                               (callset_descend_semicolon_left E CallOk) in
-         match result_a with
-         | L10.Interpret.StmtSuccess _ =>
-             interpret_stmt Ebound fc do_call builtins
-                            world' loc' b
-                            (callset_descend_semicolon_right E CallOk)
-         | _ => (world', loc', result_a)
-         end
-    | SmallStmt ss => fun E => interpret_small_stmt Ebound fc do_call builtins
-                                                    world loc ss
-                                                    (callset_descend_small_stmt E CallOk)
-    | LocalVarDecl name init scope => fun E =>
-         match map_lookup loc name with
-         | Some _ => (world, loc,
-                        L10.Interpret.StmtAbort _
-                          (L10.Interpret.AbortError "local variable already exists"))
-         | None =>
-           let '(world', result) :=
-                  interpret_expr Ebound fc do_call builtins
-                                 world loc init
-                                 (callset_descend_var_init E CallOk)
-           in match result with
-              | L10.Interpret.ExprSuccess _ value =>
-                  let '(world2, loc2, result2) :=
-                    interpret_stmt Ebound fc do_call builtins
-                                   world (map_insert loc name value) scope
-                                   (callset_descend_var_scope E CallOk)
-                  in (world2, map_remove loc2 name, result2)
-              | L10.Interpret.ExprAbort _ ab =>
-                  (world', loc, L10.Interpret.StmtAbort _ ab)
-              end
-         end
-    | IfElseStmt cond yes no => fun E => 
-        let (world', result_cond) := interpret_expr
-                                       Ebound fc do_call builtins
-                                       world loc cond
-                                       (callset_descend_stmt_if_cond E CallOk)
-        in match result_cond with
-           | L10.Interpret.ExprAbort _ ab => (world', loc, L10.Interpret.StmtAbort _ ab)
-           | L10.Interpret.ExprSuccess _ cond_value =>
-               if (Z_of_uint256 cond_value =? 0)%Z
-                 then interpret_stmt Ebound fc do_call builtins
-                                     world' loc no
-                                     (callset_descend_stmt_if_else E CallOk)
-                 else interpret_stmt Ebound fc do_call builtins
-                                     world' loc yes
-                                     (callset_descend_stmt_if_then E CallOk)
-           end
-    | Loop var start count fc_body => fun E =>
-        let (world', result_start) :=
-              interpret_expr Ebound fc do_call builtins
-                             world loc start
-                             (callset_descend_loop_start E CallOk)
-        in match result_start with
-           | L10.Interpret.ExprAbort _ ab => (world', loc, L10.Interpret.StmtAbort _ ab)
-           | L10.Interpret.ExprSuccess _ start_value =>
-              let fix interpret_loop_rec (world: world_state)
-                                         (loc: string_map uint256)
-                                         (cursor: Z)
-                                         (countdown: nat)
-                                         (name: string)
-                                         (CallOk: let _ := string_set_impl in 
-                                                  FSet.is_subset (stmt_callset fc_body)
-                                                                 (decl_callset (fun_decl fc)) = true)
-                 {struct countdown}
-                 : world_state * string_map uint256 * stmt_result uint256
-                 := match countdown with
-                    | O => (world, loc, L10.Interpret.StmtSuccess _)
-                    | S new_countdown =>
-                          let loc' := map_insert loc name (uint256_of_Z cursor) in
-                          let '(world', loc'', result) :=
-                                interpret_stmt Ebound fc do_call builtins world loc' fc_body CallOk
-                          in match result with
-                             | L10.Interpret.StmtSuccess _
-                             | L10.Interpret.StmtAbort _ L10.Interpret.AbortContinue =>
-                                 interpret_loop_rec world' loc''
-                                                    (Z.succ cursor) new_countdown name CallOk
-                             | L10.Interpret.StmtAbort _ L10.Interpret.AbortBreak =>
-                                 (world', loc'', L10.Interpret.StmtSuccess _)
-                             | _ => (world', loc'', result)
-                             end
-                    end
-               in match map_lookup loc var with
-               | Some _ => (world', loc,
-                             L10.Interpret.StmtAbort _
-                               (L10.Interpret.AbortError "loop var already exists"))
-               | None => let count_z := Z_of_uint256 count in
-                         let count_nat := Z.to_nat count_z in
-                         let start_z := Z_of_uint256 start_value in
-                         let last := (start_z + count_z - 1)%Z in
-                         if (Z_of_uint256 (uint256_of_Z last) =? last)%Z
-                           then
-                             interpret_loop_rec
-                               world' loc start_z count_nat var
-                               (callset_descend_loop_body E CallOk)
-                           else (world, loc,
-                                  L10.Interpret.StmtAbort _
-                                    (L10.Interpret.AbortError "loop range overflows"))
-               end
-           end
-    end eq_refl.
-
 Fixpoint interpret_call {call_depth_bound: nat}
                         {cd: calldag}
-                        (builtins: string -> option L10.Interpret.builtin)
+                        (builtins: string -> option builtin)
                         (fc: fun_ctx cd call_depth_bound)
                         (world: world_state)
                         (arg_values: list uint256)
@@ -521,62 +37,30 @@ Fixpoint interpret_call {call_depth_bound: nat}
 : world_state * expr_result uint256
 := match call_depth_bound as call_depth_bound' return _ = call_depth_bound' -> _ with
    | O => fun Ebound => False_rect _ (Nat.nlt_0_r (fun_depth fc)
-                                                  (eq_ind _ _ (fun_bound_ok fc) _ Ebound))
+                                                  (eq_ind _ _
+                                                          (proj1 (Nat.ltb_lt _ _) (fun_bound_ok fc))
+                                                          _ Ebound))
    | S new_call_depth_bound => fun Ebound =>
         match fun_decl fc as d return _ = d -> _ with
         | FunDecl _ arg_names body => fun E =>
-            match bind_args arg_names arg_values with
+            match L10.Interpret.bind_args arg_names arg_values with
             | inl err => (world, expr_error err)
             | inr loc =>
                 let '(world', loc', result) := interpret_stmt Ebound fc (interpret_call builtins)
                                                               builtins world loc body 
                                                               (interpret_call_helper E)
                 in (world', match result with
-                            | L10.Interpret.StmtSuccess _ => L10.Interpret.ExprSuccess _ zero256
-                            | L10.Interpret.StmtReturnFromFunction _ x => L10.Interpret.ExprSuccess _ x
-                            | L10.Interpret.StmtAbort _ a => L10.Interpret.ExprAbort _ a
+                            | StmtSuccess => ExprSuccess zero256
+                            | StmtReturnFromFunction x => ExprSuccess x
+                            | StmtAbort a => ExprAbort a
                             end)
             end
         | _ => fun _ => (world, expr_error "a declaration is found but it's not a function")
         end eq_refl
    end eq_refl.
 
-Local Lemma make_fun_ctx_helper {cd: calldag}
-                          {name: string}
-                          {d : decl}
-                          (Ed : cd_declmap cd name = Some d)
-                          (Edepth : cd_depthmap cd name = None):
-  False.
-Proof.
-assert (W := cd_depthmap_ok cd name).
-unfold cd_declmap in Ed.
-rewrite Ed in W.
-unfold cd_depthmap in Edepth.
-rewrite Edepth in W. exact W.
-Qed.
-
-Definition make_fun_ctx_and_bound (cd: calldag)
-                                  (name: string)
-: option { bound: nat & fun_ctx cd bound }
-:= match cd_declmap cd name as maybe_d return _ = maybe_d -> _ with
-   | None => fun _ => None
-   | Some d => fun Ed =>
-      match cd_depthmap cd name as depth' return _ = depth' -> _ with
-      | None => fun Edepth => False_rect _ (make_fun_ctx_helper Ed Edepth)
-      | Some depth => fun Edepth => Some (existT _
-                                                 (S depth)
-                                                 {| fun_name := name
-                                                  ; fun_decl := d
-                                                  ; fun_decl_ok := Ed
-                                                  ; fun_depth := depth
-                                                  ; fun_depth_ok := Edepth
-                                                  ; fun_bound_ok := Nat.lt_succ_diag_r _
-                                                 |})
-      end eq_refl
-   end eq_refl.
-
 (** This is a simplified interface to interpret_call that takes care of creating a function context. *)
-Definition interpret (builtins: string -> option L10.Interpret.builtin)
+Definition interpret (builtins: string -> option builtin)
                      (cd: calldag)
                      (function_name: string)
                      (world: world_state)
