Calldag.v
@@ -1,0 +1,88 @@
+From Coq Require Import String Arith.
+From Vyper Require Import Config.
+
+Record generic_calldag {C: VyperConfig} (decl_type: Type) (callset: decl_type -> string_set) := {
+  cd_declmap:  string -> option decl_type;
+  cd_depthmap: string -> option nat;
+  cd_depthmap_ok:
+    forall name: string,
+      match cd_declmap name with
+      | None => True
+      | Some decl =>
+          match cd_depthmap name with
+          | None => False
+          | Some x =>
+              let _ := string_set_impl in
+              FSet.for_all (callset decl)
+                           (fun callee => match cd_depthmap callee with
+                                          | None => false
+                                          | Some y => y <? x
+                                          end)
+               = true
+            end
+      end;
+}.
+Arguments cd_declmap {C decl_type callset}.
+Arguments cd_depthmap {C decl_type callset}.
+Arguments cd_depthmap_ok {C decl_type callset}.
+
+(**
+  A functional context is the result of looking up a function by name in a calldag.
+ *)
+Record fun_ctx {C: VyperConfig}
+               {decl_type: Type}
+               {decl_callset: decl_type -> string_set}
+               (cd: generic_calldag decl_type decl_callset)
+               (bound: nat) := {
+  fun_name: string;
+  fun_depth: nat;
+  fun_depth_ok: cd_depthmap cd fun_name = Some fun_depth;
+  fun_decl: decl_type;
+  fun_decl_ok: cd_declmap cd fun_name = Some fun_decl;
+  fun_bound_ok: fun_depth <? bound = true;
+}.
+Arguments fun_name     {C _ _ _ _}.
+Arguments fun_depth    {C _ _ _ _}.
+Arguments fun_depth_ok {C _ _ _ _}.
+Arguments fun_decl     {C _ _ _ _}.
+Arguments fun_decl_ok  {C _ _ _ _}.
+Arguments fun_bound_ok {C _ _ _ _}.
+
+Local Lemma make_fun_ctx_helper {C: VyperConfig}
+                                {decl_type: Type}
+                                {decl_callset: decl_type -> string_set}
+                                {cd: generic_calldag decl_type decl_callset}
+                                {name: string}
+                                {d: decl_type}
+                                (Ed: cd_declmap cd name = Some d)
+                                (Edepth: cd_depthmap cd name = None):
+  False.
+Proof.
+assert (W := cd_depthmap_ok cd name).
+rewrite Ed in W. rewrite Edepth in W. exact W.
+Qed.
+
+(** Create a function context from scratch (meaning that there's no pre-existing bound). *)
+Definition make_fun_ctx_and_bound {C: VyperConfig}
+                                  {decl_type: Type}
+                                  {decl_callset: decl_type -> string_set}
+                                  (cd: generic_calldag decl_type decl_callset)
+                                  (name: string)
+: option { bound: nat & fun_ctx cd bound }
+:= match cd_declmap cd name as maybe_d return _ = maybe_d -> _ with
+   | None => fun _ => None
+   | Some d => fun Ed =>
+      match cd_depthmap cd name as depth' return _ = depth' -> _ with
+      | None => fun Edepth => False_rect _ (make_fun_ctx_helper Ed Edepth)
+      | Some depth => fun Edepth => Some (existT _
+                                                 (S depth)
+                                                 {| fun_name := name
+                                                  ; fun_decl := d
+                                                  ; fun_decl_ok := Ed
+                                                  ; fun_depth := depth
+                                                  ; fun_depth_ok := Edepth
+                                                  ; fun_bound_ok := proj2 (Nat.ltb_lt _ _)
+                                                                          (Nat.lt_succ_diag_r _)
+                                                 |})
+      end eq_refl
+   end eq_refl.
