L10/Interpret.v
@@ -1,5 +1,5 @@
 From Coq Require Import String Arith NArith ZArith Eqdep_dec.
-From Vyper Require Import Config.
+From Vyper Require Import Config Calldag.
 From Vyper.L10 Require Import AST Base Callset Descend Expr Stmt.
 From Vyper Require FSet Map UInt256.
 
@@ -8,6 +8,29 @@ Local Open Scope string_scope.
 
 Section Interpret.
 Context {C: VyperConfig}.
+
+(** Initialize a map of local variables with argument names and argument values. *)
+Fixpoint bind_args (names: list string) (values: list uint256)
+: string + string_map uint256
+:= let _ := string_map_impl in
+   match names with
+   | nil => match values with
+            | nil => inr Map.empty
+            | _ => inl "function called with too many arguments"
+            end
+   | hn :: tn => match values with
+                 | nil => inl "function called with too few arguments"
+                 | hv :: tv =>
+                     match bind_args tn tv with
+                     | inl err => inl err
+                     | inr bindings =>
+                        match Map.lookup bindings hn with
+                        | Some _ => inl "error: duplicate variable name"
+                        | None => inr (Map.insert bindings hn hv)
+                        end
+                     end
+                 end
+   end.
 
 Local Lemma interpret_call_helper {this_decl: decl}
                                   {fun_name: string}
@@ -52,38 +75,6 @@ Fixpoint interpret_call {call_depth_bound: nat}
       end eq_refl
   end eq_refl.
 
-Local Lemma make_fun_ctx_helper {cd: calldag}
-                          {name: string}
-                          {d : decl}
-                          (Ed : cd_declmap cd name = Some d)
-                          (Edepth : cd_depthmap cd name = None):
-  False.
-Proof.
-assert (W := cd_depthmap_ok cd name).
-rewrite Ed in W. rewrite Edepth in W. exact W.
-Qed.
-
-Definition make_fun_ctx_and_bound (cd: calldag)
-                                  (name: string)
-: option { bound: nat & fun_ctx cd bound }
-:= match cd_declmap cd name as maybe_d return _ = maybe_d -> _ with
-   | None => fun _ => None
-   | Some d => fun Ed =>
-      match cd_depthmap cd name as depth' return _ = depth' -> _ with
-      | None => fun Edepth => False_rect _ (make_fun_ctx_helper Ed Edepth)
-      | Some depth => fun Edepth => Some (existT _
-                                                 (S depth)
-                                                 {| fun_name := name
-                                                  ; fun_decl := d
-                                                  ; fun_decl_ok := Ed
-                                                  ; fun_depth := depth
-                                                  ; fun_depth_ok := Edepth
-                                                  ; fun_bound_ok := proj2 (Nat.ltb_lt _ _)
-                                                                          (Nat.lt_succ_diag_r _)
-                                                 |})
-      end eq_refl
-   end eq_refl.
-
 (** This is a simplified interface to interpret_call that takes care of creating a function context. *)
 Definition interpret (builtins: string -> option builtin)
                      (cd: calldag)
@@ -95,36 +86,5 @@ Definition interpret (builtins: string -> option builtin)
    | None => (world, expr_error "declaration not found")
    | Some (existT _ bound fc) => interpret_call builtins fc world arg_values
    end.
-
-(*
-
-Lemma interpret_stmt_fun_ctx_irrel {bigger_call_depth_bound smaller_call_depth_bound: nat}
-                                   (Ebound: bigger_call_depth_bound = S smaller_call_depth_bound)
-                                   {cd: calldag}
-                                   {fc1 fc2: fun_ctx cd bigger_call_depth_bound}
-                                   (FcOk: fun_name fc1 = fun_name fc2)
-                                   (do_call: forall
-                                                 (fc': fun_ctx cd smaller_call_depth_bound)
-                                                 (world: world_state)
-                                                 (arg_values: list uint256),
-                                               world_state * expr_result uint256)
-                                   (builtins: string -> option builtin)
-                                   (world: world_state)
-                                   (loc: string_map uint256)
-                                   (s: stmt)
-                                   (NotLocVar: is_local_var_decl s = false)
-                                   (CallOk1: let _ := string_set_impl in 
-                                                FSet.is_subset (stmt_callset s)
-                                                               (decl_callset (fun_decl fc1))
-                                                = true)
-                                   (CallOk2: let _ := string_set_impl in 
-                                                FSet.is_subset (stmt_callset s)
-                                                               (decl_callset (fun_decl fc2))
-                                                = true):
-  interpret_stmt Ebound fc1 do_call builtins world loc s NotLocVar CallOk1
-   =
-  interpret_stmt Ebound fc2 do_call builtins world loc s NotLocVar CallOk2.
-Proof.
-*)
 
 End Interpret.
