L20/Expr.v
@@ -1,0 +1,163 @@
+From Coq Require Import ZArith String.
+
+From Vyper Require Import Config Calldag.
+
+From Vyper.L10 Require Import Base.
+
+From Vyper.L20 Require Import AST Callset Descend.
+
+
+Fixpoint interpret_expr {C: VyperConfig}
+                        {bigger_call_depth_bound smaller_call_depth_bound: nat}
+                        (Ebound: bigger_call_depth_bound = S smaller_call_depth_bound)
+                        {cd: calldag}
+                        (fc: fun_ctx cd bigger_call_depth_bound)
+                        (do_call: forall
+                                      (fc': fun_ctx cd smaller_call_depth_bound)
+                                      (world: world_state)
+                                      (arg_values: list uint256),
+                                    world_state * expr_result uint256)
+                        (builtins: string -> option builtin)
+                        (world: world_state)
+                        (loc: string_map uint256)
+                        (e: expr)
+                        (CallOk: let _ := string_set_impl in 
+                                   FSet.is_subset (expr_callset e)
+                                                  (decl_callset (fun_decl fc))
+                                   = true)
+{struct e}
+: world_state * expr_result uint256
+:= let fix interpret_expr_list (world: world_state)
+                               (loc: string_map uint256)
+                               (e: list expr)
+                               (CallOk: let _ := string_set_impl in 
+                                        FSet.is_subset (expr_list_callset e)
+                                                       (decl_callset (fun_decl fc))
+                                        = true)
+      {struct e}
+      : world_state * expr_result (list uint256)
+      := match e as e' return e = e' -> _ with
+         | nil => fun _ => (world, ExprSuccess nil)
+         | (h :: t)%list => fun E =>
+             let (world', result_h) := interpret_expr Ebound fc do_call builtins
+                                                      world loc h
+                                                      (callset_descend_head E CallOk)
+             in match result_h with
+                | ExprAbort ab => (world', ExprAbort ab)
+                | ExprSuccess x =>
+                   let (world'', result_t) := interpret_expr_list world' loc t
+                                                                  (callset_descend_tail E CallOk)
+                   in (world'', match result_t with
+                                | ExprAbort _ => result_t
+                                | ExprSuccess y => ExprSuccess (x :: y)%list
+                                end)
+                 end
+         end eq_refl
+    in match e as e' return e = e' -> _ with
+       | Const val => fun _ => (world, ExprSuccess val)
+       | LocalVar name => fun _ =>
+           (world, match map_lookup loc name with
+                   | Some val => ExprSuccess val
+                   | None => expr_error "Local variable not found"
+                   end)
+       | StorageVar name => fun _ => 
+           (world, match storage_lookup world name with
+                   | Some val => ExprSuccess val
+                   | None => expr_error "Storage variable not found"
+                   end)
+       | UnOp op a => fun E =>
+           let (world', result) := interpret_expr Ebound fc do_call builtins
+                                                  world loc a
+                                                  (callset_descend_unop E CallOk)
+           in (world', match result with
+                       | ExprSuccess val => interpret_unop op val
+                       | ExprAbort _ => result
+                       end)
+       | BinOp op a b => fun E =>
+           let (world', result_a) := interpret_expr Ebound fc do_call builtins
+                                                    world loc a
+                                                    (callset_descend_binop_left E CallOk)
+           in match result_a with
+           | ExprAbort _ => (world', result_a)
+           | ExprSuccess x =>
+             let (world'', result_b) := interpret_expr Ebound fc do_call builtins
+                                                       world' loc b
+                                                       (callset_descend_binop_right E CallOk)
+             in (world'', match result_b with
+                          | ExprAbort _ => result_b
+                          | ExprSuccess y => interpret_binop op x y
+                          end)
+           end
+       | IfThenElse cond yes no => fun E =>
+           let (world', result_cond) := interpret_expr Ebound fc do_call builtins
+                                                       world loc cond
+                                                       (callset_descend_if_cond E CallOk)
+           in match result_cond with
+              | ExprAbort _ => (world', result_cond)
+              | ExprSuccess cond_value =>
+                  if (Z_of_uint256 cond_value =? 0)%Z
+                    then interpret_expr Ebound fc do_call builtins
+                                        world' loc no
+                                        (callset_descend_if_else E CallOk)
+                    else interpret_expr Ebound fc do_call builtins
+                                        world' loc yes
+                                        (callset_descend_if_then E CallOk)
+              end
+       | LogicalAnd a b => fun E =>
+           let (world', result_a) := interpret_expr Ebound fc do_call builtins
+                                                    world loc a
+                                                    (callset_descend_and_left E CallOk)
+           in match result_a with
+              | ExprAbort _ => (world', result_a)
+              | ExprSuccess a_value =>
+                  if (Z_of_uint256 a_value =? 0)%Z
+                    then (world', result_a)
+                    else interpret_expr Ebound fc do_call builtins
+                                        world' loc b
+                                        (callset_descend_and_right E CallOk)
+              end
+       | LogicalOr a b => fun E =>
+           let (world', result_a) := interpret_expr Ebound fc do_call builtins
+                                                    world loc a
+                                                    (callset_descend_or_left E CallOk)
+           in match result_a with
+              | ExprAbort msg => (world', result_a)
+              | ExprSuccess a_value =>
+                  if (Z_of_uint256 a_value =? 0)%Z
+                    then interpret_expr Ebound fc do_call builtins
+                                        world' loc b
+                                        (callset_descend_or_right E CallOk)
+                    else (world', result_a)
+              end
+       | PrivateCall name args => fun E =>
+           let (world', result_args) :=
+             interpret_expr_list world loc args
+                                 (callset_descend_args E CallOk)
+           in match result_args with
+              | ExprAbort ab => (world', ExprAbort ab)
+              | ExprSuccess arg_values =>
+                  match fun_ctx_descend fc CallOk Ebound E with
+                  | None => (* can't resolve the function, maybe it's a builtin *)
+                            (world', expr_error "can't resolve function name")
+                  | Some new_fc => do_call new_fc world' arg_values
+                  end
+              end
+       | BuiltinCall name args => fun E =>
+           let (world', result_args) :=
+             interpret_expr_list world loc args
+                                 (callset_descend_builtin_args E CallOk)
+           in match result_args with
+              | ExprAbort ab => (world', ExprAbort ab)
+              | ExprSuccess arg_values =>
+                match builtins name with
+                | Some (existT _ arity b) =>
+                   (if (arity =? List.length arg_values)%nat as arity_ok 
+                    return _ = arity_ok -> _
+                        then fun Earity =>
+                               call_builtin arg_values Earity (b world')
+                        else fun _ => (world', expr_error "builtin with wrong arity"))
+                      eq_refl
+                | None => (world', expr_error "can't resolve function name")
+                end
+              end
+       end eq_refl.
