L20/Stmt.v
@@ -1,0 +1,182 @@
+From Coq Require Import ZArith String.
+
+From Vyper Require Import Config Calldag.
+
+From Vyper.L10 Require Import Base.
+
+From Vyper.L20 Require Import AST Callset Descend Expr.
+
+Section Stmt.
+Context {C: VyperConfig}.
+
+Definition interpret_small_stmt {bigger_call_depth_bound smaller_call_depth_bound: nat}
+                                (Ebound: bigger_call_depth_bound = S smaller_call_depth_bound)
+                                {cd: calldag}
+                                (fc: fun_ctx cd bigger_call_depth_bound)
+                                (do_call: forall
+                                              (fc': fun_ctx cd smaller_call_depth_bound)
+                                              (world: world_state)
+                                              (arg_values: list uint256),
+                                            world_state * expr_result uint256)
+                                (builtins: string -> option builtin)
+                                (world: world_state)
+                                (loc: string_map uint256)
+                                (s: small_stmt)
+                                (CallOk: let _ := string_set_impl in 
+                                         FSet.is_subset (small_stmt_callset s)
+                                                        (decl_callset (fun_decl fc))
+                                         = true)
+: world_state * string_map uint256 * stmt_result uint256
+:= match s as s' return s = s' -> _ with
+   | Pass     => fun _ => (world, loc, StmtSuccess)
+   | Abort ab => fun _ => (world, loc, StmtAbort ab)
+   | Return e => fun E =>
+        let (world', result) := interpret_expr Ebound fc do_call builtins
+                                               world loc e
+                                               (callset_descend_return E CallOk)
+        in (world', loc, match result with
+                         | ExprSuccess value => StmtReturnFromFunction value
+                         | ExprAbort ab => StmtAbort ab
+                         end)
+   | Raise e => fun E =>
+        let (world', result) := interpret_expr Ebound fc do_call builtins
+                                               world loc e
+                                               (callset_descend_raise E CallOk)
+        in (world', loc, StmtAbort (match result with
+                                    | ExprSuccess value => AbortException value
+                                    | ExprAbort ab      => ab
+                                    end))
+   | Assign lhs rhs => fun E =>
+        let (world', result) := interpret_expr Ebound fc do_call builtins
+                                               world loc rhs
+                                               (callset_descend_assign_rhs E CallOk)
+        in do_assign world' loc lhs result
+   | ExprStmt e => fun E =>
+                   let (world', result) := interpret_expr Ebound fc do_call builtins
+                                                          world loc e
+                                                          (callset_descend_expr_stmt E CallOk)
+                   in (world', loc, match result with
+                                    | ExprSuccess a => StmtSuccess
+                                    | ExprAbort ab => StmtAbort ab
+                                    end)
+   end eq_refl.
+
+Fixpoint interpret_stmt {bigger_call_depth_bound smaller_call_depth_bound: nat}
+                        (Ebound: bigger_call_depth_bound = S smaller_call_depth_bound)
+                        {cd: calldag}
+                        (fc: fun_ctx cd bigger_call_depth_bound)
+                        (do_call: forall
+                                      (fc': fun_ctx cd smaller_call_depth_bound)
+                                      (world: world_state)
+                                      (arg_values: list uint256),
+                                    world_state * expr_result uint256)
+                        (builtins: string -> option builtin)
+                        (world: world_state)
+                        (loc: string_map uint256)
+                        (s: stmt)
+                        (CallOk: let _ := string_set_impl in 
+                                 FSet.is_subset (stmt_callset s)
+                                                (decl_callset (fun_decl fc)) = true)
+ {struct s}
+ : world_state * string_map uint256 * stmt_result uint256
+ := match s as s' return s = s' -> _ with
+    | Semicolon a b => fun E =>
+         let '(world', loc', result_a) :=
+                interpret_stmt Ebound fc do_call builtins
+                               world loc a
+                               (callset_descend_semicolon_left E CallOk) in
+         match result_a with
+         | StmtSuccess =>
+             interpret_stmt Ebound fc do_call builtins
+                            world' loc' b
+                            (callset_descend_semicolon_right E CallOk)
+         | _ => (world', loc', result_a)
+         end
+    | SmallStmt ss => fun E => interpret_small_stmt Ebound fc do_call builtins
+                                                    world loc ss
+                                                    (callset_descend_small_stmt E CallOk)
+    | LocalVarDecl name init scope => fun E =>
+         match map_lookup loc name with
+         | Some _ => (world, loc, StmtAbort (AbortError "local variable already exists"))
+         | None =>
+           let '(world', result) :=
+                  interpret_expr Ebound fc do_call builtins
+                                 world loc init
+                                 (callset_descend_var_init E CallOk)
+           in match result with
+              | ExprSuccess value =>
+                  let '(world2, loc2, result2) :=
+                    interpret_stmt Ebound fc do_call builtins
+                                   world (map_insert loc name value) scope
+                                   (callset_descend_var_scope E CallOk)
+                  in (world2, map_remove loc2 name, result2)
+              | ExprAbort ab =>
+                  (world', loc, StmtAbort ab)
+              end
+         end
+    | IfElseStmt cond yes no => fun E => 
+        let (world', result_cond) := interpret_expr
+                                       Ebound fc do_call builtins
+                                       world loc cond
+                                       (callset_descend_stmt_if_cond E CallOk)
+        in match result_cond with
+           | ExprAbort ab => (world', loc, StmtAbort ab)
+           | ExprSuccess cond_value =>
+               if (Z_of_uint256 cond_value =? 0)%Z
+                 then interpret_stmt Ebound fc do_call builtins
+                                     world' loc no
+                                     (callset_descend_stmt_if_else E CallOk)
+                 else interpret_stmt Ebound fc do_call builtins
+                                     world' loc yes
+                                     (callset_descend_stmt_if_then E CallOk)
+           end
+    | Loop var start count fc_body => fun E =>
+        let (world', result_start) :=
+              interpret_expr Ebound fc do_call builtins
+                             world loc start
+                             (callset_descend_loop_start E CallOk)
+        in match result_start with
+           | ExprAbort ab => (world', loc, StmtAbort ab)
+           | ExprSuccess start_value =>
+              let fix interpret_loop_rec (world: world_state)
+                                         (loc: string_map uint256)
+                                         (cursor: Z)
+                                         (countdown: nat)
+                                         (name: string)
+                                         (CallOk: let _ := string_set_impl in 
+                                                  FSet.is_subset (stmt_callset fc_body)
+                                                                 (decl_callset (fun_decl fc)) = true)
+                 {struct countdown}
+                 : world_state * string_map uint256 * stmt_result uint256
+                 := match countdown with
+                    | O => (world, loc, StmtSuccess)
+                    | S new_countdown =>
+                          let loc' := map_insert loc name (uint256_of_Z cursor) in
+                          let '(world', loc'', result) :=
+                                interpret_stmt Ebound fc do_call builtins world loc' fc_body CallOk
+                          in match result with
+                             | StmtSuccess | StmtAbort AbortContinue =>
+                                 interpret_loop_rec world' loc''
+                                                    (Z.succ cursor) new_countdown name CallOk
+                             | StmtAbort AbortBreak =>
+                                 (world', loc'', StmtSuccess)
+                             | _ => (world', loc'', result)
+                             end
+                    end
+               in match map_lookup loc var with
+               | Some _ => (world', loc, StmtAbort (AbortError "loop var already exists"))
+               | None => let count_z := Z_of_uint256 count in
+                         let count_nat := Z.to_nat count_z in
+                         let start_z := Z_of_uint256 start_value in
+                         let last := (start_z + count_z - 1)%Z in
+                         if (Z_of_uint256 (uint256_of_Z last) =? last)%Z
+                           then
+                             interpret_loop_rec
+                               world' loc start_z count_nat var
+                               (callset_descend_loop_body E CallOk)
+                           else (world, loc, StmtAbort (AbortError "loop range overflows"))
+               end
+           end
+    end eq_refl.
+
+End Stmt.
